seems not working

src/tools/parallelcomposition/event_systemsScript.sml
@@ -1,6 +1,7 @@
 open HolKernel Parse boolLib bossLib;
 open sumTheory;
 open pred_setTheory;
+open listTheory;
 
 val _ = new_theory "event_systems";
 
@@ -21,7 +22,6 @@ val _ = Datatype `transitionsystem_t = <|
   sys_dedu   : ('pred) deduction_t
                          |>`;
 
-
 (* reach a state *)
 Inductive reach:
 [~init:]
@@ -37,20 +37,59 @@ Definition invariant:
   (invariant ES I ⇔ (∀v p s. (reach ES (v,p,s)) ==> I (v,p,s)))
 End        
 
+
+(* trace *)
+val _ = Parse.type_abbrev("trace_t", ``:'event list``);
+
+Definition trace:
+  ((trace ES (v,p,s) [] (v',p',s')) = ((v,p,s) = (v',p',s'))) ∧
+  ((trace ES (v,p,s) (e::(t: 'event trace_t)) (v'',p'',s'')) =
+         (∀v' p' s'. (trace ES (v,p,s) t (v',p',s')) ∧ (ES.sys_trans (v',p',s') e (v'',p'',s''))))
+End
 (*
-Theorem Invariant_rule:
- ∀I ES. (∀v0 p0 s0. (ES.sys_init (v0,p0,s0)) ⇒ I (v0,p0,s0)) ∧ (∀v p s e v' p' s'. (ES.sys_trans (v,p,s) e (v',p',s')) /\ (reach ES (v,p,s)) ∧ (I (v,p,s)) ⇒ I (v',p',s')) ⇒ invariant ES I
+Inductive trace:
+[~nil:]
+  (!(ES :('event, 'pred, 'state, 'symb) transitionsystem_t) (v:'symb set) (p: 'pred set) (s: 'state).
+     (trace ES (v,p,s) [] (v,p,s))) ∧
+[~snoc:]
+  !(ES :('event, 'pred, 'state, 'symb) transitionsystem_t) v p s.
+      (trace ES (v,p,s) (t: 'event trace_t) (v',p',s')) ∧ (ES.sys_trans (v',p',s') e (v'',p'',s'')) ==> (trace ES (v,p,s) (t ⧺ [e]) (v'',p'',s''))
+End
+*)    
+
+Theorem trace_independence:
+ ∀(ES :('event, 'pred, 'state, 'symb) transitionsystem_t) (FS :('event, 'pred, 'state, 'symb) transitionsystem_t) v p s t v' p' s'. (trace ES (v,p,s) t (v',p',s')) ∧ (ES.sys_trans = FS.sys_trans) ⇒ (trace FS (v,p,s) t (v',p',s'))
 Proof
-  rewrite_tac [invariant] >> rpt strip_tac >> ...
+  rpt strip_tac >>
+Induct_on `t` >>
+          asm_rewrite_tac [trace] >>
+          gen_tac >>
+          asm_rewrite_tac [trace] >>
+          rpt strip_tac >>
+  PAT_X_ASSUM ``∀v''' p''' s'''. A`` (ASSUME_TAC o (Q.SPECL [`v'''`,`p'''`,`s'''`])) >>
+                       METIS_TAC [trace]
+              
+QED
+                                                  
+Theorem trace_single:
+ ∀ES v p s e v' p' s'. (ES.sys_trans (v,p,s) e (v',p',s')) ⇒ (trace ES (v,p,s) [e] (v',p',s'))
+Proof
+  rpt strip_tac >>
+      `[e] = ([] ⧺ [e] ` by (rewrite_tac [APPEND_EQ_SING])
+      Cases_on `[e] = ([] ⧺ [e])` 
+          rewrite_tac [APPEND_EQ_SING]
+      asm_rewrite_tac [trace_nil,trace_snoc]
 PAT_X_ASSUM ``∀v p s e v' p' s'. A`` (ASSUME_TAC o (Q.SPECL [`v`,`p`,`s`,`e`,`v'`,`p'`,`s'`]))
                  PAT_X_ASSUM ``∀v0 p0 s0. A`` (ASSUME_TAC o (Q.SPECL [`v0`,`p0`,`s0`]))
                                    rewrite_tac [invariant,reach_trans,reach_init]
                                    rpt gen_tac
                                    IMP_RES_TAC(reach_trans)
-                                         IMP_RES_TAC(reach_init)
+                                         IMP_RES_TAC(APPEND_EQ_SING)
                                    PAT_X_ASSUM ``∀v' p' s' e. A`` (ASSUME_TAC o (Q.SPECL [`v'`,`p'`,`s'`,`e`]))
-                                                        RES_TAC
+                                                     RES_TAC
+
+                                                     FULL_SIMP_TAC (list_ss++pred_setSimps.PRED_SET_ss++boolSimps.LIFT_COND_ss++boolSimps.EQUIV_EXTRACT_ss) [trace_nil,trace_snoc]
+                                                     METIS_TAC [trace]
 QED
-*)
         
 val _ = export_theory();
